Phi_Semantics/PhiSem_Mem_C_Ag_NT.thy
@@ -2,7 +2,19 @@ theory PhiSem_Mem_C_Ag_NT \<comment> \<open>Named Tuple\<close>
   imports PhiSem_Mem_C PhiSem_Aggregate_Named_Tuple
 begin
 
+section \<open>Named Tuple in Memory\<close>
 
+subsection \<open>Semantics\<close>
+
+debt_axiomatization
+    Map_of_Val_ntup: \<open>Map_of_Val (V_named_tup.mk vs) =
+      (\<lambda>path. case path of AgIdx_S s # path' \<Rightarrow>
+                                if s |\<in>| fmdom vs then Map_of_Val (the (fmlookup vs s)) path'
+                                                  else 1
+                         | _ \<Rightarrow> 1)\<close>
+
+
+subsection \<open>Syntax\<close>
 
 syntax "\<phi>_shared_named_tuple_" :: \<open>logic \<Rightarrow> \<phi>_symbol_ \<Rightarrow> logic \<Rightarrow> \<phi>_tuple_arg_\<close> ("_ \<odiv> _: _")
 
@@ -48,6 +60,78 @@ term \<open>a \<odiv> b\<close>
 term \<open>\<m>\<e>\<m>[addr] \<lbrace> c \<odiv> a: T, dd \<odiv> b: \<lbrace> e: U \<rbrace>\<rbrace>\<close>
 term \<open>\<m>\<e>\<m>[addr] \<lbrace> a: T, b: (U \<^emph> D)\<rbrace>\<close>
 *)
+
+subsection \<open>Reasoning\<close>
+
+subsubsection \<open>ToA Mapper\<close>
+
+text \<open>The following lemma cannot be automated because it is tightly related to the semantics\<close>
+
+lemma Mem_Coerce_NTup:
+  \<open> (\<m>\<e>\<m>-\<c>\<o>\<e>\<r>\<c>\<e> \<lbrace> SYMBOL_VAR(s): T \<rbrace>) = (AgIdx_S s \<^bold>\<rightarrow>\<^sub># \<m>\<e>\<m>-\<c>\<o>\<e>\<r>\<c>\<e> T) \<close>
+  apply (rule \<phi>Type_eqI_BI; unfold BI_eq_iff; clarsimp; rule; clarsimp)
+  subgoal for x v
+    by (rule exI[where x=\<open>to_share \<circ> map_option discrete \<circ> Map_of_Val v\<close>],
+        auto simp add: Map_of_Val_ntup fun_eq_iff push_map_cons_neq
+             split: aggregate_index'.split list.split)
+  subgoal for x v
+    by (rule exI[where x=\<open>V_named_tup.mk (fmupd s v fmempty)\<close>],
+        auto simp add: Map_of_Val_ntup fun_eq_iff push_map_cons_neq
+             split: aggregate_index'.split list.split) .
+
+lemma Mem_Coerce_NTup_Comb:
+  \<open> Fx |\<inter>| Fy = {||}
+\<Longrightarrow> Is_Named_Tuple T Fx
+\<Longrightarrow> Is_Named_Tuple U Fy
+\<Longrightarrow> \<m>\<e>\<m>-\<c>\<o>\<e>\<r>\<c>\<e> (T \<^emph> U) = \<m>\<e>\<m>-\<c>\<o>\<e>\<r>\<c>\<e> T \<^emph> \<m>\<e>\<m>-\<c>\<o>\<e>\<r>\<c>\<e> U \<close>
+  apply (rule \<phi>Type_eqI_BI, unfold BI_eq_iff Is_Named_Tuple_def Premise_def;
+      clarsimp; rule; clarsimp)
+
+  subgoal premises prems for x y a b
+    by (insert prems(2)[THEN spec, THEN spec, THEN mp, OF prems(5)]
+               prems(3)[THEN spec, THEN spec, THEN mp, OF prems(4)],
+        clarsimp simp: V_named_tup_mult Map_of_Val_ntup,
+        rule exI[where x=\<open>to_share \<circ> map_option discrete \<circ> Map_of_Val a\<close>],
+        rule exI[where x=\<open>to_share \<circ> map_option discrete \<circ> Map_of_Val b\<close>],
+        insert prems(1,4-), auto simp: Map_of_Val_ntup
+          fun_eq_iff times_fun sep_disj_fun_def split: list.split aggregate_index'.split,
+        rule exI[where x=a], (auto simp: Map_of_Val_ntup)[1],
+        rule exI[where x=b], (auto simp: Map_of_Val_ntup)[1])
+  
+  subgoal premises prems for x y a b
+    apply (insert prems(2)[THEN spec, THEN spec, THEN mp, OF prems(6)]
+                  prems(3)[THEN spec, THEN spec, THEN mp, OF prems(5)])
+    apply (rule exI[where x=\<open>a * b\<close>])
+    apply (insert prems(1,4-), auto simp: V_named_tup_mult Map_of_Val_ntup
+        fun_eq_iff times_fun sep_disj_fun_def split: list.split aggregate_index'.split)
+    by (metis V_named_tup_mult V_named_tup_sep_disj inf.commute) .
+
+
+lemma [\<phi>reason %\<phi>mapToA_norm]:
+  \<open> Is_Named_Tuple U\<^sub>2  field\<^sub>2
+\<Longrightarrow> Is_Named_Tuple U\<^sub>2' field\<^sub>2
+\<Longrightarrow> \<c>\<o>\<n>\<d>\<i>\<t>\<i>\<o>\<n>[\<s>\<a>\<f>\<e>] fmdom tys = field\<^sub>2 \<and> s |\<notin>| field\<^sub>2
+
+\<Longrightarrow> \<m>\<a>\<p> g : (AgIdx_S s \<^bold>\<rightarrow>\<^sub># \<m>\<e>\<m>-\<c>\<o>\<e>\<r>\<c>\<e>[ty] U\<^sub>1 \<^emph> \<m>\<e>\<m>-\<c>\<o>\<e>\<r>\<c>\<e>[semty_ntup tys] U\<^sub>2) \<^emph>[C\<^sub>R] R
+          \<mapsto> (AgIdx_S s \<^bold>\<rightarrow>\<^sub># \<m>\<e>\<m>-\<c>\<o>\<e>\<r>\<c>\<e>[ty] U\<^sub>1' \<^emph> \<m>\<e>\<m>-\<c>\<o>\<e>\<r>\<c>\<e>[semty_ntup tys] U\<^sub>2') \<^emph>[C\<^sub>R] R
+    \<o>\<v>\<e>\<r> f : T \<^emph>[C\<^sub>W] W \<mapsto> T' \<^emph>[C\<^sub>W] W'
+    \<w>\<i>\<t>\<h> \<g>\<e>\<t>\<t>\<e>\<r> getter \<s>\<e>\<t>\<t>\<e>\<r> setter \<i>\<n> D
+
+\<Longrightarrow> \<m>\<a>\<p> g : \<m>\<e>\<m>-\<c>\<o>\<e>\<r>\<c>\<e>[semty_ntup (fmupd s ty tys)] (\<lbrace> SYMBOL_VAR(s): U\<^sub>1 \<rbrace> \<^emph> U\<^sub>2) \<^emph>[C\<^sub>R] R
+          \<mapsto> \<m>\<e>\<m>-\<c>\<o>\<e>\<r>\<c>\<e>[semty_ntup (fmupd s ty tys)] (\<lbrace> SYMBOL_VAR(s): U\<^sub>1' \<rbrace> \<^emph> U\<^sub>2') \<^emph>[C\<^sub>R] R
+    \<o>\<v>\<e>\<r> f : T \<^emph>[C\<^sub>W] W \<mapsto> T' \<^emph>[C\<^sub>W] W'
+    \<w>\<i>\<t>\<h> \<g>\<e>\<t>\<t>\<e>\<r> getter \<s>\<e>\<t>\<t>\<e>\<r> setter \<i>\<n> D \<close>
+
+  unfolding Guided_Mem_Coercion_def Transformation_def Premise_def
+  subgoal premises prems proof -
+    have t1: \<open>{|s|} |\<inter>| field\<^sub>2 = {||}\<close>
+      using prems(3) by blast
+    show ?thesis
+      by (unfold Mem_Coerce_NTup_Comb[where T=\<open>\<lbrace> SYMBOL_VAR(s): U\<^sub>1 \<rbrace>\<close> and U=\<open>U\<^sub>2\<close>, OF t1 Is_Named_Tuple_sing prems(1)]
+                 Mem_Coerce_NTup_Comb[where T=\<open>\<lbrace> SYMBOL_VAR(s): U\<^sub>1' \<rbrace>\<close> and U=\<open>U\<^sub>2'\<close>, OF t1 Is_Named_Tuple_sing prems(2)]
+                 Mem_Coerce_NTup,
+          insert prems(4), this)
+  qed .
 
 
 end
