Phi_Semantics/PhiSem_Mem_C_Tuple.thy
@@ -3,7 +3,10 @@ theory PhiSem_Mem_C_Tuple
 begin
 
 debt_axiomatization
-    Map_of_Val_tup: \<open>Map_of_Val (V_tup.mk vs) = nnode (map Map_of_Val vs)\<close>
+    Map_of_Val_tup: \<open>Map_of_Val (V_tup.mk vs) =
+      (\<lambda>path. case path of AgIdx_N i # path' \<Rightarrow> if i < length vs then Map_of_Val (vs!i) path'
+                                                else 1
+                         | _ \<Rightarrow> 1)\<close>
 
 
 end
